src/tls/test/TestClient.fst
@@ -194,8 +194,8 @@ let main host port =
   let rid = new_region root in
   let log = HandshakeLog.create #rid in
 
-  let ks = KeySchedule.create #rid Client in
-  let cr, _ = KeySchedule.ks_client_init_12 ks in  
+  let ks, cr = KeySchedule.create #rid Client in
+  let _ = KeySchedule.ks_client_init_12 ks in  
   let ch = Handshake.prepareClientHello config ks None None in
 
   let pv = ch.ch_protocol_version in 
